src/Lean/Meta/Basic.lean
@@ -1321,7 +1321,7 @@ private def getDefInfoTemp (info : ConstantInfo) : MetaM (Option ConstantInfo) :
    `constName` is an instance. This difference should be irrelevant for `isClassQuickConst?`. -/
 private def getConstTemp? (constName : Name) : MetaM (Option ConstantInfo) := do
   match (← getEnv).find? constName with
-  | some (info@(ConstantInfo.thmInfo _))  => getTheoremInfo info
+  | some (ConstantInfo.thmInfo _)          => return none
   | some (info@(ConstantInfo.defnInfo _)) => getDefInfoTemp info
   | some info                             => pure (some info)
   | none                                  => throwUnknownConstantAt (← getRef) constName
